Classes/Except.v
@@ -1,4 +1,17 @@
-Class Except (M : Type -> Type) := {
+Require Export Base.
+Require Import Classes.Applicative.
+Require Import Classes.Monad.
+
+Class Except (M : Type -> Type) `{Monad M} := {
   throw    : M unit;
   trycatch : M unit -> M unit -> M unit;
+  bind_fail : forall (f : unit -> M unit), bindM throw f = throw;
+  trycatch_throw_left : forall (x : M unit), 
+    trycatch throw x = x;
+  trycatch_throw_right : forall (x : M unit),
+    trycatch x throw = x;
+  trycatch_pure : forall x h, trycatch (pure x) h = pure x;
 }.
+
+Hint Rewrite @trycatch_throw_left @trycatch_throw_right 
+  @trycatch_pure : soundness.
