Instances/IsNat/Nat.v
@@ -5,28 +5,33 @@ Require Import Language.Statements.
 Require Import Types.State.
 Require Import Types.Result.
 Require Import Instances.Monad.
+Require Import Classes.Applicative.
 
-Definition ensure_nat (v : cvalue) : State nat :=
+Definition ensure_nat (v : cvalue) : ConcreteState nat :=
   match v with
-  | VNat x => Just _ (return_state x)
-  | _ => None _
+  | VNat x => pure_maybeT _ (pure x)
+  | _ => pure None 
   end.
 
-Definition extract_natM (n : nat) : State nat :=
-  Just _ (return_state n).
+Definition extract_natM (n : nat) : ConcreteState nat :=
+  pure_maybeT _ (pure n).
 
-Definition plusM (n m : nat) : State nat := Just _ (returnM (plus n m)).
+Definition plusM (n m : nat) : ConcreteState nat := 
+  pure_maybeT _ (pure (plus n m)).
 
-Definition multM (n m : nat) : State nat := Just _ (returnM (mult n m)).
+Definition multM (n m : nat) : ConcreteState nat := 
+  pure_maybeT _ (pure (mult n m)).
 
-Definition eqbM (n m : nat) : State bool := Just _ (returnM (Nat.eqb n m)).
+Definition eqbM (n m : nat) : ConcreteState bool := 
+  pure_maybeT _ (pure (Nat.eqb n m)).
 
-Definition lebM (n m : nat) : State bool := Just _ (returnM (Nat.leb n m)).
+Definition lebM (n m : nat) : ConcreteState bool := 
+  pure_maybeT _ (pure (Nat.leb n m)).
 
-Definition build_natural (n : nat) : State cvalue := 
-  Just _ (returnM (VNat n)).
+Definition build_natural (n : nat) : ConcreteState cvalue := 
+  pure_maybeT _ (pure (VNat n)).
 
-Global Instance nat_numerical : IsNat State cvalue bool nat :=
+Global Instance nat_numerical : IsNat ConcreteState cvalue bool nat :=
 {
   ensure_nat := ensure_nat;
   build_nat := build_natural;
