Instances/Monad.v
@@ -2,7 +2,7 @@ Require Export Base.
 Require Import Coq.Program.Basics.
 Require Import Classes.Applicative.
 Require Import Classes.Functor.
-Require Import Classes.Monad.
+Require Export Classes.Monad.
 Require Import FunctionalExtensionality.
 Require Import Language.Statements.
 Require Import Types.Maps.
@@ -13,6 +13,13 @@ Inductive Maybe (A : Type) : Type :=
 Arguments Just {_}.
 Arguments None {_}.
 
+Ltac solve_monad := repeat (simple_solve;
+  match goal with
+  | |- bindM ?f _ = ?f => rewrite <- bind_id_right; f_equal
+  | |- bindM ?f _ = bindM ?f _ => apply bind_equiv_r
+  | _ => simple_solve
+  end).
+
 Section Maybe_Functor.
   Definition fmap_maybe {A B : Type} (f : A -> B) (ma : Maybe A) : Maybe B :=
     match ma with
@@ -20,17 +27,14 @@ Section Maybe_Functor.
     | None => None
     end.
   Arguments fmap_maybe [_ _] _ _.
+  Hint Unfold fmap_maybe : soundness.
 
   Lemma fmap_maybe_id : ∀ A : Type, fmap_maybe (@id A) = id.
-  Proof.
-    intros. extensionality m. destruct m; reflexivity.
-  Qed.
+  Proof. simple_solve. Qed.
 
   Lemma fmap_maybe_compose : ∀ (A B C : Type) (f : A → B) (g : B → C),
     fmap_maybe (f ∘ g) = fmap_maybe f ∘ fmap_maybe g.
-  Proof.
-    intros. unfold compose. extensionality m. destruct m; reflexivity.
-  Qed.
+  Proof. simple_solve. Qed.
 
   Global Instance functor_maybe : Functor (Maybe) := 
   {
@@ -39,6 +43,7 @@ Section Maybe_Functor.
     fmap_compose := fmap_maybe_compose;
   }.
 End Maybe_Functor.
+Hint Rewrite fmap_maybe_id fmap_maybe_compose : soundness.
 
 Section Maybe_Applicative.
   Definition app_maybe {A B : Type} 
@@ -49,34 +54,27 @@ Section Maybe_Applicative.
     | Just f, Just x => Just (f x)
     end.
   Arguments app_maybe [_ _] _ _.
+  Hint Unfold app_maybe : soundness.
 
   Lemma app_maybe_id : 
     ∀ (A : Type) (f : Maybe A), app_maybe (Just id) f = f.
-  Proof.
-    intros. destruct f; reflexivity.
-  Qed.
+  Proof. simple_solve. Qed.
 
   Lemma app_maybe_homomorphism :
     ∀ (A B : Type) (f : A → B) (x : A), 
     app_maybe (Just f) (Just x) = Just (f x).
-  Proof.
-    reflexivity.
-  Qed.
+  Proof. simple_solve. Qed.
 
   Lemma app_maybe_interchange :
     ∀ (A B : Type) (u : Maybe (A → B)) (y : A),
     app_maybe u (Just y) = app_maybe (Just (λ f : A → B, f y)) u.
-  Proof.
-    destruct u; reflexivity.
-  Qed.
+  Proof. simple_solve. Qed.
 
   Lemma app_maybe_compose :
     ∀ (A B C : Type) (u : Maybe (B → C)) (v : Maybe (A → B)) (w : Maybe A),
     app_maybe (app_maybe (app_maybe (Just compose) u) v) w =
     app_maybe u (app_maybe v w).
-  Proof.
-    destruct u, v, w; reflexivity.
-  Qed.
+  Proof. simple_solve. Qed.
 
   Global Instance applicative_maybe : Applicative Maybe :=
   {
@@ -88,6 +86,7 @@ Section Maybe_Applicative.
     app_compose := app_maybe_compose;
   }.
 End Maybe_Applicative.
+Hint Rewrite app_maybe_id app_maybe_homomorphism : soundness.
 
 Section Maybe_Monad.
   Definition bind_maybe {A B : Type} 
@@ -97,19 +96,20 @@ Section Maybe_Monad.
     | Just a => k a
     end.
   Arguments bind_maybe [_ _].
+  Hint Unfold bind_maybe : soundness.
 
   Lemma bind_maybe_id_left : ∀ (A B : Type) (f : A → Maybe B) (a : A), 
     bind_maybe (Just a) f = f a.
-  Proof. reflexivity. Qed.
+  Proof. simple_solve. Qed.
 
   Lemma bind_maybe_id_right : ∀ (A : Type) (MA : Maybe A), 
     bind_maybe MA Just = MA.
-  Proof. destruct MA; reflexivity. Qed.
+  Proof. simple_solve. Qed.
 
   Lemma bind_maybe_assoc : ∀ (A B C : Type) (MA : Maybe A) 
     (f : A → Maybe B) (g : B → Maybe C),
   bind_maybe (bind_maybe MA f) g = bind_maybe MA (λ a : A, bind_maybe (f a) g).
-  Proof. destruct MA; reflexivity. Qed.
+  Proof. simple_solve. Qed.
 
   Global Instance monad_maybe : Monad Maybe :=
   {
@@ -118,8 +118,8 @@ Section Maybe_Monad.
     bind_id_right := bind_maybe_id_right;
     bind_assoc := bind_maybe_assoc;
   }.
-
 End Maybe_Monad.
+Hint Rewrite bind_maybe_id_left bind_maybe_id_right : soundness.
 
 Inductive AbstractMaybe (A : Type) : Type :=
   | JustA : A -> AbstractMaybe A
@@ -138,17 +138,14 @@ Section AbstractMaybe_Functor.
     | NoneA => NoneA
     end. 
   Arguments fmap_abstract_maybe [_ _] _ _.
+  Hint Unfold fmap_abstract_maybe : soundness.
 
   Lemma fmap_abstract_maybe_id : ∀ A : Type, fmap_abstract_maybe (@id A) = id.
-  Proof. 
-    intros. extensionality m. destruct m; reflexivity.
-  Qed.
+  Proof. simple_solve. Qed.
 
   Lemma fmap_abstract_maybe_compose : ∀ (A B C : Type) (f : A → B) (g : B → C),
   fmap_abstract_maybe (f ∘ g) = fmap_abstract_maybe f ∘ fmap_abstract_maybe g.
-  Proof.
-    intros. unfold compose. extensionality m. destruct m; reflexivity.
-  Qed.
+  Proof. simple_solve. Qed.
 
   Global Instance functor_abstract_maybe : Functor AbstractMaybe :=
   {
@@ -157,6 +154,7 @@ Section AbstractMaybe_Functor.
     fmap_compose := fmap_abstract_maybe_compose;
   }.
 End AbstractMaybe_Functor.
+Hint Rewrite fmap_abstract_maybe_id fmap_abstract_maybe_compose : soundness.
 
 Section AbstractMaybe_Applicative.
   Definition app_abstract_maybe {A B : Type} (Mf : AbstractMaybe (A -> B))
@@ -170,20 +168,21 @@ Section AbstractMaybe_Applicative.
   | JustA f, JustA a => JustA (f a)
   end.
   Arguments app_abstract_maybe [_ _] _ _.
+  Hint Unfold app_abstract_maybe : soundness.
 
   Lemma app_abstract_maybe_id : ∀ (A : Type) (f : AbstractMaybe A),
     app_abstract_maybe (JustA id) f = f.
-  Proof. destruct f; reflexivity. Qed.
+  Proof. simple_solve. Qed.
 
   Lemma app_abstract_maybe_homomorphism : ∀ (A B : Type) (f : A → B) (x : A),
   app_abstract_maybe (JustA f) (JustA x) = JustA (f x).
-  Proof. reflexivity. Qed.
+  Proof. simple_solve. Qed.
 
   Lemma app_abstract_maybe_interchange : ∀ (A B : Type) 
     (u : AbstractMaybe (A → B)) (y : A),
     app_abstract_maybe u (JustA y) =
     app_abstract_maybe (JustA (λ f : A → B, f y)) u.
-  Proof. reflexivity. Qed.
+  Proof. simple_solve. Qed.
 
   Lemma app_abstract_maybe_compose : ∀ (A B C : Type) 
     (u : AbstractMaybe (B → C)) (v : AbstractMaybe (A → B)) 
@@ -191,9 +190,7 @@ Section AbstractMaybe_Applicative.
     app_abstract_maybe
       (app_abstract_maybe (app_abstract_maybe (JustA compose) u) v) w =
     app_abstract_maybe u (app_abstract_maybe v w).
-  Proof.
-    intros. unfold compose. destruct u, v, w; reflexivity.
-  Qed.
+  Proof. simple_solve. Qed.
 
   Global Instance applicative_abstract_maybe : Applicative AbstractMaybe :=
   {
@@ -205,6 +202,7 @@ Section AbstractMaybe_Applicative.
     app_compose := app_abstract_maybe_compose;
   }.
 End AbstractMaybe_Applicative.
+Hint Resolve app_abstract_maybe_id app_abstract_maybe_homomorphism : soundness.
 
 Section AbstractMaybe_Monad.
   Definition bind_maybeA {A B : Type}
@@ -219,23 +217,21 @@ Section AbstractMaybe_Monad.
                        end
     end.
   Arguments bind_maybeA [_].
+  Hint Unfold bind_maybeA : soundness.
 
   Lemma bind_maybeA_id_left : ∀ (A B : Type) (f : A → AbstractMaybe B) (a : A),
   bind_maybeA B (JustA a) f = f a.
-  Proof. reflexivity. Qed.
+  Proof. simple_solve. Qed.
 
   Lemma bind_maybeA_id_right :  ∀ (A : Type) (MA : AbstractMaybe A),
     bind_maybeA A MA JustA = MA.
-  Proof. destruct MA; reflexivity. Qed.
+  Proof. simple_solve. Qed.
 
   Lemma bind_maybeA_assoc : ∀ (A B C : Type) (MA : AbstractMaybe A) 
     (f : A → AbstractMaybe B) (g : B → AbstractMaybe C),
     bind_maybeA C (bind_maybeA B MA f) g =
     bind_maybeA C MA (λ a : A, bind_maybeA C (f a) g).
-  Proof.
-    intros. destruct MA; [reflexivity|simpl|reflexivity].
-    destruct (f a); [simpl|simpl|reflexivity]; destruct (g b); reflexivity.
-  Qed.
+  Proof. simple_solve. Qed.
 
   Global Instance monad_abstract_maybe : Monad AbstractMaybe :=
   {
@@ -245,28 +241,24 @@ Section AbstractMaybe_Monad.
     bind_assoc := bind_maybeA_assoc;
   }.
 End AbstractMaybe_Monad.
+Hint Rewrite bind_maybeA_id_left bind_maybeA_id_right : soundness.
 
 Definition MaybeT (M : Type -> Type) (A : Type) : Type := M (Maybe A).
 
 Section MaybeT_Functor.
-  Context (M : Type -> Type) `{Monad M}.
+  Context {M : Type -> Type} `{Monad M}.
 
   Definition fmap_maybeT {A B : Type} (f : A -> B)
-    (m : MaybeT M A) : MaybeT M B :=  fmap (fmap_maybe f) m. 
+    (m : MaybeT M A) : MaybeT M B :=  fmap (fmap (F:=Maybe) f) m. 
   Arguments fmap_maybeT [_ _] _ _.
+  Hint Unfold fmap_maybeT : soundness.
 
   Lemma fmap_maybeT_id : ∀ A : Type, fmap_maybeT (@id A) = id.
-  Proof.
-    intros. unfold fmap_maybeT. extensionality m.
-    rewrite fmap_maybe_id, fmap_id. reflexivity.
-  Qed.
+  Proof. simple_solve. Qed.
 
   Lemma fmap_maybeT_compose : ∀ (A B C : Type) (f : A → B) (g : B → C),
   fmap_maybeT (f ∘ g) = fmap_maybeT f ∘ fmap_maybeT g.
-  Proof. 
-    intros. extensionality m. unfold fmap_maybeT. 
-    rewrite fmap_maybe_compose. rewrite fmap_compose. reflexivity.
-  Qed.
+  Proof. simple_solve. Qed.
 
   Global Instance functor_maybeT : Functor (MaybeT M) :=
   {
@@ -276,66 +268,41 @@ Section MaybeT_Functor.
   }.
 End MaybeT_Functor.
 
+Hint Rewrite fmap_maybeT_id fmap_maybeT_compose : soundness.
+
 Section MaybeT_Applicative.
-  Context (M : Type -> Type) `{inst : Monad M}.
+  Context {M : Type -> Type} `{inst : Monad M}.
 
   Definition pure_maybeT {A : Type} (x : A) :  M (Maybe A) :=
     pure (Just x).
   Arguments pure_maybeT [_] _.
+  Hint Unfold pure_maybeT : soundness.
 
   Definition app_maybeT {A B : Type} (Mmf : M (Maybe (A -> B)))
     (Mma : M (Maybe A)) : M (Maybe B) :=
-    @bindM _ _ _ _ (Maybe (A -> B)) (Maybe B) Mmf (fun mf =>
-    @bindM _ _ _ _ (Maybe A) (Maybe B) Mma (fun ma =>
+    bindM Mmf (fun mf =>
+    bindM Mma (fun ma =>
       pure (app_maybe mf ma))).
   Arguments app_maybeT [_ _] _ _.
+  Hint Unfold app_maybeT : soundness.
 
   Lemma app_maybeT_id : ∀ (A : Type) (f : M (Maybe A)),
     app_maybeT (pure_maybeT id) f = f.
-  Proof.
-    intros. unfold pure_maybeT. unfold app_maybeT.
-    rewrite bind_id_left. 
-    assert ((λ ma : Maybe A, pure (app_maybe (Just id) ma)) = (λ ma : Maybe A,
-    (pure ma))).
-    extensionality m. rewrite app_maybe_id. reflexivity.
-    rewrite H1; clear H1.
-    assert ((λ ma : Maybe A, pure ma) = pure).
-    extensionality x. reflexivity.
-    rewrite H1; clear H1.  unfold MaybeT in f.
-    apply bind_id_right.
-  Qed.
+  Proof. solve_monad. Qed.
 
   Lemma app_maybeT_homomorphism : ∀ (A B : Type) (f : A → B) (x : A),
   app_maybeT (pure_maybeT f) (pure_maybeT x) = pure_maybeT (f x).
-  Proof. 
-    intros. unfold pure_maybeT. unfold app_maybeT. repeat rewrite bind_id_left.
-    rewrite app_maybe_homomorphism. reflexivity.
-  Qed.
+  Proof. solve_monad. Qed.
 
   Lemma app_maybeT_interchange : ∀ (A B : Type) (u : MaybeT M (A → B)) (y : A),
   app_maybeT u (pure_maybeT y) = app_maybeT (pure_maybeT (λ f : A → B, f y)) u.
-  Proof. 
-    intros. unfold pure_maybeT. unfold app_maybeT. rewrite bind_id_left.
-    assert ((λ mf : Maybe (A → B), bindM (pure (Just y)) (λ ma : Maybe A, pure
-    (app_maybe mf ma))) = (λ ma : Maybe (A → B), pure (app_maybe (Just (λ f : A
-    -> B, f y)) ma))).
-    - extensionality mf. simpl. destruct mf; rewrite bind_id_left; reflexivity.
-    - rewrite H1. reflexivity.
-  Qed.
+  Proof. solve_monad. Qed.
 
   Lemma app_maybeT_compose : ∀ (A B C : Type) (u : MaybeT M (B → C)) 
     (v : MaybeT M (A → B))  (w : MaybeT M A),
     app_maybeT (app_maybeT (app_maybeT (pure_maybeT compose) u) v) w =
     app_maybeT u (app_maybeT v w).
-  Proof.
-    intros. unfold app_maybeT, pure_maybeT.
-    rewrite bind_id_left. repeat rewrite bind_assoc. 
-    apply bind_equiv_r. extensionality m. rewrite bind_id_left.
-    simpl. repeat rewrite bind_assoc. apply bind_equiv_r.
-    extensionality m'. rewrite bind_id_left. rewrite bind_assoc.
-    apply bind_equiv_r. extensionality m''. rewrite bind_id_left.
-    destruct m, m', m''; reflexivity.
-  Qed.
+  Proof. solve_monad. Qed.
 
   Global Instance applicative_maybeT : Applicative (MaybeT M) :=
   {
@@ -347,9 +314,11 @@ Section MaybeT_Applicative.
     app_compose := app_maybeT_compose;
   }.
 End MaybeT_Applicative.
+Hint Unfold pure_maybeT app_maybeT : soundness.
+Hint Rewrite app_maybeT_id app_maybeT_homomorphism : soundness.
 
 Section MaybeT_Monad.
-  Context (M : Type -> Type) `{inst : Monad M}.
+  Context {M : Type -> Type} `{inst : Monad M}.
 
   Definition bind_maybeT {A B : Type} (Mma : M (Maybe A))
     (f : A -> M (Maybe B)) : M (Maybe B) :=
@@ -360,34 +329,21 @@ Section MaybeT_Monad.
       end
     ).
   Arguments bind_maybeT [_ _] _ _.
+  Hint Unfold bind_maybeT : soundness.
 
   Lemma bind_maybeT_id_left : ∀ (A B : Type) (f : A → MaybeT M B) (a : A), 
     bind_maybeT (pure a) f = f a.
-  Proof.
-    intros. simpl. unfold pure_maybeT, bind_maybeT. 
-    rewrite bind_id_left. reflexivity.
-  Qed.
+  Proof. solve_monad. Qed.
 
   Lemma bind_maybeT_id_right : ∀ (A : Type) (MA : MaybeT M A),
     bind_maybeT MA pure = MA.
-  Proof.
-    intros. simpl. unfold pure_maybeT, bind_maybeT. 
-    assert ((λ ma : Maybe A,
-     match ma with | Just a => pure (Just a) | None => pure None end) = 
-     λ ma : Maybe A, pure ma). extensionality m; destruct m;
-     reflexivity. rewrite H1; clear H1. apply bind_id_right.
-  Qed.
+  Proof. solve_monad. Qed.
 
   Lemma bind_maybeT_assoc : ∀ (A B C : Type) (MA : MaybeT M A) 
     (f : A → MaybeT M B) (g : B → MaybeT M C),
     bind_maybeT (bind_maybeT MA f) g =
     bind_maybeT MA (λ a : A, bind_maybeT (f a) g).
-  Proof.
-    intros. unfold bind_maybeT, pure_maybeT. repeat rewrite bind_assoc.
-    apply bind_equiv_r. extensionality m. destruct m.
-    - reflexivity. 
-    - rewrite bind_id_left. reflexivity.
-  Qed.
+  Proof. solve_monad. Qed.
 
   Global Instance monad_maybeT : Monad (MaybeT M) :=
   {
@@ -397,9 +353,11 @@ Section MaybeT_Monad.
     bind_assoc := bind_maybeT_assoc;
   }.
 End MaybeT_Monad.
+Hint Unfold bind_maybeT : soundness.
+Hint Rewrite bind_maybeT_id_left bind_maybeT_id_right : soundness.
 
 Section MaybeT_MonadT.
-  Context (M : Type -> Type) `{Monad M}.
+  Context {M : Type -> Type} `{Monad M}.
   
   Definition lift_maybeT {A : Type} (Ma : M A) : M (Maybe A) :=
     fmap Just Ma.
@@ -414,79 +372,54 @@ End MaybeT_MonadT.
 Definition MaybeAT (M : Type -> Type) (A : Type) : Type := M (AbstractMaybe A).
 
 Section MaybeAT_Functor.
-  Context (M : Type -> Type) `{Monad M}.
+  Context {M : Type -> Type} `{inst : Functor M}.
 
   Definition fmap_maybeAT {A B : Type} 
     (f : A -> B) (Ma : MaybeAT M A) : MaybeAT M B :=
     fmap (fmap_abstract_maybe f) Ma.
   Arguments fmap_maybeAT [_ _] _ _.
+  Hint Unfold fmap_maybeAT : soundness.
 
   Global Instance functor_maybeAT : Functor (MaybeAT M) :=
   {
     fmap := fmap_maybeAT;
-  }.
-  - intros. unfold fmap_maybeAT. extensionality Ma. 
-    rewrite fmap_abstract_maybe_id. rewrite fmap_id. reflexivity.
-  - intros. extensionality m. unfold fmap_maybeAT.
-    rewrite fmap_abstract_maybe_compose. rewrite fmap_compose.
-    reflexivity.
-  Defined.
+  }. all: solve_monad. Defined.
 End MaybeAT_Functor.
 
 Section MaybeAT_Applicative.
-  Context (M : Type -> Type) `{Monad M}.
+  Context {M : Type -> Type} `{inst : Monad M}.
 
-  Definition pure_maybeAT {A : Type} (x : A) : M (AbstractMaybe A) :=
+  Definition pure_maybeAT {A : Type} (x : A) : MaybeAT M A :=
     pure (JustA x).
   Arguments pure_maybeAT [_] _.
+  Hint Unfold pure_maybeAT : soundness.
 
   Definition app_maybeAT {A B : Type} (Mmf : M (AbstractMaybe (A -> B)))
     (Mma : M (AbstractMaybe A)) : M (AbstractMaybe B) :=
-    @bindM _ _ _ _ (AbstractMaybe (A -> B)) (AbstractMaybe B) Mmf (fun mf =>
-    @bindM _ _ _ _ (AbstractMaybe A) (AbstractMaybe B) Mma (fun ma =>
+    bindM Mmf (fun mf : AbstractMaybe (A -> B) =>
+    bindM Mma (fun ma : AbstractMaybe A =>
       pure (app_abstract_maybe mf ma))).
   Arguments app_maybeAT [_ _] _ _.
+  Hint Unfold app_maybeAT : soundness.
 
   Lemma app_maybeAT_id : ∀ (A : Type) (f : MaybeAT M A), 
     app_maybeAT (pure_maybeAT id) f = f.
-  Proof.
-    intros. unfold app_maybeAT, pure_maybeAT. rewrite bind_id_left.
-    assert ((λ ma : AbstractMaybe A, pure (app_abstract_maybe (JustA id) ma)) =
-             λ ma : AbstractMaybe A, pure ma).
-    { extensionality m. destruct m; reflexivity. }
-    rewrite H2; clear H2.
-    apply bind_id_right.
-  Qed.
-
+  Proof. solve_monad. Qed.
 
   Lemma app_maybeAT_homomorphism : ∀ (A B : Type) (f : A → B) (x : A),
     app_maybeAT (pure_maybeAT f) (pure_maybeAT x) = pure_maybeAT (f x).
-  Proof.
-    intros. unfold app_maybeAT, pure_maybeAT. repeat rewrite bind_id_left.
-    rewrite app_abstract_maybe_homomorphism. reflexivity.
-  Qed.
+  Proof. solve_monad. Qed.
 
   Lemma app_maybeAT_interchange : ∀ (A B : Type) (u : MaybeAT M (A → B)) (y : A),
     app_maybeAT u (pure_maybeAT y) = 
     app_maybeAT (pure_maybeAT (λ f : A → B, f y)) u.
-  Proof.
-    intros. unfold pure_maybeAT, app_maybeAT. rewrite bind_id_left.
-    apply bind_equiv_r. extensionality x. rewrite bind_id_left.
-    destruct x; reflexivity.
-  Qed.
+  Proof. solve_monad. Qed.
 
   Lemma app_maybeAT_compose : ∀ (A B C : Type) 
     (u : MaybeAT M (B → C)) (v : MaybeAT M (A → B)) (w : MaybeAT M A),
     app_maybeAT (app_maybeAT (app_maybeAT (pure_maybeAT compose) u) v) w =
     app_maybeAT u (app_maybeAT v w).
-  Proof.
-    intros. unfold app_maybeAT, pure_maybeAT.
-    rewrite bind_id_left. repeat rewrite bind_assoc. apply bind_equiv_r.
-    extensionality a. rewrite bind_id_left. repeat rewrite bind_assoc.
-    apply bind_equiv_r. extensionality b. rewrite bind_id_left.
-    repeat rewrite bind_assoc. apply bind_equiv_r. extensionality c.
-    rewrite bind_id_left. destruct a, b, c; reflexivity.
-  Qed.
+  Proof. solve_monad. Qed.
 
   Global Instance applicative_maybeAT : Applicative (MaybeAT M) :=
   {
@@ -498,10 +431,10 @@ Section MaybeAT_Applicative.
     app_compose := app_maybeAT_compose;
   }.
 End MaybeAT_Applicative.
+Hint Unfold pure_maybeAT app_maybeAT : soundness.
 
-Require Import Classes.Joinable.
 Section MaybeAT_Monad.
-  Context (M : Type -> Type) `{Monad M}.
+  Context {M : Type -> Type} `{Monad M}.
 
   Definition bind_maybeAT {A B} 
     (Mma : M (AbstractMaybe A))
@@ -519,46 +452,21 @@ Section MaybeAT_Monad.
                        end)
     end).
   Arguments bind_maybeAT [_ _].
+  Hint Unfold bind_maybeAT : soundness.
 
   Lemma bind_maybeAT_id_left : ∀ (A B : Type) (f : A → MaybeAT M B) (a : A), 
     bind_maybeAT (pure a) f = f a.
-  Proof.
-    intros. simpl. unfold bind_maybeAT, pure_maybeAT. rewrite bind_id_left.
-    reflexivity.
-  Qed.
+  Proof. solve_monad. Qed.
 
   Lemma bind_maybeAT_id_right : ∀ (A : Type) (MA : MaybeAT M A), 
     bind_maybeAT MA pure = MA.
-  Proof.
-    intros. simpl. unfold bind_maybeAT, pure_maybeAT. simpl.
-    assert ((λ ma : AbstractMaybe A,
-     match ma with | JustA a => pure (JustA a) | JustOrNoneA a =>
-         bindM (pure (JustA a))
-           (λ mfa : AbstractMaybe A,
-              match mfa with
-              | JustA b | JustOrNoneA b => pure (JustOrNoneA b)
-              | NoneA => pure NoneA
-              end) | NoneA => pure NoneA
-     end) = (λ ma, pure ma)).
-     extensionality ma. destruct ma; try reflexivity. rewrite bind_id_left.
-     reflexivity.
-     rewrite H2. rewrite bind_id_right. reflexivity.
-  Qed.
+  Proof. solve_monad. Qed.
 
   Lemma bind_maybeAT_assoc : ∀ (A B C : Type) (MA : MaybeAT M A) 
     (f : A → MaybeAT M B) (g : B → MaybeAT M C),
     bind_maybeAT (bind_maybeAT MA f) g =
     bind_maybeAT MA (λ a : A, bind_maybeAT (f a) g).
-  Proof.
-    intros. unfold bind_maybeAT. repeat rewrite bind_assoc. apply bind_equiv_r.
-    extensionality a. destruct a.
-    - apply bind_equiv_r. reflexivity.
-    - repeat rewrite bind_assoc. apply bind_equiv_r. extensionality b.
-      destruct b; repeat rewrite bind_id_left; try reflexivity.
-      repeat rewrite bind_assoc. apply bind_equiv_r.
-      extensionality c. destruct c; rewrite bind_id_left; reflexivity.
-    - rewrite bind_id_left. reflexivity.
-  Qed.
+  Proof. solve_monad. Qed.
 
   Global Instance monad_maybeAT 
   : Monad (MaybeAT M) :=
@@ -568,11 +476,10 @@ Section MaybeAT_Monad.
     bind_id_right := bind_maybeAT_id_right;
     bind_assoc := bind_maybeAT_assoc;
   }.
-
 End MaybeAT_Monad.
 
 Section MaybeAT_MonadT.
-  Context (M : Type -> Type) `{Monad M}.
+  Context {M : Type -> Type} `{Monad M}.
 
   Definition lift_maybeAT {A : Type} (Ma : M A) : MaybeAT M A :=
     fmap JustA Ma.
@@ -592,18 +499,12 @@ Section State_Functor.
     (f : A -> B) (Fa : State S A) : State S B :=
   fun st => let (x, s) := Fa st in (f x, s).
   Arguments fmap_state [_ _ _] _ _.
+  Hint Unfold fmap_state : soundness.
 
   Global Instance functor_state (S : Type) : Functor (State S) :=
   {
     fmap := @fmap_state S;
-  }.
-  - intros. apply functional_extensionality. intros. 
-    apply functional_extensionality. intros. unfold id.
-    unfold fmap_state. destruct (x x0) eqn:Hx. reflexivity.
-  - intros. apply functional_extensionality. intros.
-    apply functional_extensionality. intros. unfold compose.
-    unfold fmap_state. destruct (x x0). reflexivity.
-  Defined.
+  }. all: solve_monad. Defined.
 
 End State_Functor.
 
@@ -615,20 +516,13 @@ Section State_Applicative.
     (Mf : State S (A -> B)) (Ma : State S A) : State S B :=
     fun st => let (f, st') := Mf st in 
               let (a, st'') := Ma st' in (f a, st'').
+  Hint Unfold pure_state app_state : soundness.
 
   Global Instance applicative_state (S : Type) : Applicative (State S) :=
   {
     pure := @pure_state S;
     app := @app_state S;
-  }.
-  - intros. apply functional_extensionality.
-    intros. unfold pure_state, app_state. destruct (f x). unfold id.
-    reflexivity.
-  - unfold pure_state, app_state. reflexivity.
-  - unfold pure_state, app_state. reflexivity.
-  - unfold pure_state, app_state. intros. apply functional_extensionality.
-    intros. destruct (u x), (v s), (w s0). reflexivity.
-  Defined.
+  }. all: simple_solve. Defined.
 End State_Applicative.
 
 Section State_Monad.
@@ -637,19 +531,78 @@ Section State_Monad.
     fun st => match (p st) with
               | (x, st') => k x st'
               end.
+  Hint Unfold bind_state : soundness.
 
   Global Instance monad_state (S : Type) :  Monad (State S) :=
   {
     bindM := @bind_state S;
-  }.
-  - intros. apply functional_extensionality.
-    intros. unfold pure_state, bind_state; reflexivity.
-  - intros. unfold bind_state, pure_state. apply functional_extensionality.
-    intros. destruct (MA x). reflexivity.
-  - intros. unfold bind_state. apply functional_extensionality. intros.
-    destruct (MA x); reflexivity.
-  Defined.
+  }. all: simple_solve. Defined.
 End State_Monad.
 
+Definition StateT (S : Type) (M : Type -> Type) (A : Type) : Type :=
+  S -> M (A*S)%type.
 
-  
+Section Functor_StateT.
+  Context {M : Type -> Type} `{Monad M}.
+
+  Definition fmap_stateT (S : Type) {A B} (f : A -> B) (m : StateT S M A)
+    : StateT S M B :=
+    fun s : S => bindM (m s) 
+      (fun x => let (a, s') := x : (A*S)%type in pure (f a, s')).
+  Hint Unfold fmap_stateT : soundness.
+
+  Global Instance functor_stateT (S : Type) : Functor (StateT S M) :=
+  {
+    fmap := @fmap_stateT S;
+  }. all: solve_monad. Defined.
+End Functor_StateT.
+
+Section Applicative_StateT.
+  Context {M : Type -> Type} `{Monad M}.
+
+  Definition pure_stateT (S : Type) {A : Type} (x : A) : StateT S M A :=
+    fun s => pure (x, s).
+
+  Definition app_stateT
+    (S : Type) {A B : Type}
+    (sf : StateT S M (A -> B)) (sa : StateT S M A) : StateT S M B :=
+    fun st : S =>
+    bindM (sf st) (fun '(f, stf) =>
+      bindM (sa stf) (fun '(a, sta) =>
+        pure (f a, sta))).
+  Hint Unfold pure_stateT app_stateT : soundness.
+
+  Global Instance applicative_stateT (S : Type) : Applicative (StateT S M) :=
+  {
+    pure := @pure_stateT S;
+    app := @app_stateT S;
+  }. all: solve_monad. Defined.
+End Applicative_StateT.
+Hint Unfold pure_stateT app_stateT : soundness.
+
+Section Monad_StateT.
+  Context {M : Type -> Type} `{Monad M}.
+
+  Definition bind_stateT (S : Type) {A B : Type} 
+    (MA : StateT S M A) (f : A -> StateT S M B) : StateT S M B :=
+    fun st => bindM (MA st) (fun '(a, st') => f a st').
+  Hint Unfold bind_stateT : soundness.
+
+  Global Instance monad_stateT (S : Type) : Monad (StateT S M) :=
+  {
+    bindM := @bind_stateT S;
+  }. all: solve_monad. Defined.
+End Monad_StateT.
+
+Section MonadT_StateT.
+  Context {M : Type -> Type} `{Monad M}.
+
+  Definition lift_stateT (S : Type) {A : Type} (MA : M A) : StateT S M A :=
+    fun st => bindM MA (fun a => pure (a, st)).
+
+  Global Instance monadT_stateT (S : Type) : MonadT (StateT S) :=
+  {
+    liftT := @lift_stateT S;
+  }.
+End MonadT_StateT.
+
