Instances/Store/ConcreteStore.v
@@ -1,18 +1,49 @@
 Require Import Types.Maps.
+Require Import Types.Stores.
 Require Import Language.Statements.
 Require Import Classes.Store.
 Require Import Types.State.
 Require Import Types.Result.
 Require Import Types.Stores.
 Require Import Instances.Monad.
+Require Import Classes.Monad.
+Require Import Classes.Applicative.
+Require Import Classes.Functor.
 
-Definition store_get (x : string) : State cvalue := 
-  Just _ (fun st => (st x, st)).
+Section store_stateT. 
+  Context (M : Type -> Type) `{Monad M}.
 
-Definition store_put (x : string) (v : cvalue) : State unit := 
-  Just _ (fun st => (tt, (t_update st x v))).
+  Definition stateT_get (S : Type) := fun s : S => pure(s, s).
 
-Instance store_concrete : Store State cvalue := {
-  get := store_get;
-  put := store_put;
-}.
+  Definition stateT_put (S : Type) := fun s : S => fun _ : S => pure(tt, s).
+
+  Global Instance store_stateT (S : Type) : 
+  Store S (StateT S M) (inst:=monad_stateT S) :=
+  {
+    get := @stateT_get S;
+    put := @stateT_put S;
+  }.
+End store_stateT.
+
+Section store_maybeT.
+  Context {M : Type -> Type} `{inst : Monad M}.
+
+  Global Instance store_maybeT (S : Type) `{Store S M} :
+  Store S (MaybeT M) :=
+  {
+    get := fmap Just get;
+    put := fun s => put s ;; pure (Just tt);
+  }.
+
+End store_maybeT.
+
+Section store_maybeAT.
+  Context {M : Type -> Type} `{inst : Monad M}.
+
+  Global Instance store_maybeAT (S : Type) `{Store S M} :
+  Store S (MaybeAT M) :=
+  {
+    get := fmap JustA get;
+    put := fun s => put s ;; pure (JustA tt);
+  }.
+End store_maybeAT.
