Types/State.v
@@ -5,102 +5,28 @@ Require Import Classes.PreorderedSet.
 Require Import Instances.Joinable.
 Require Import Instances.Preorder.
 Require Import Language.Statements.
+Require Import Classes.Functor.
+Require Import Classes.Applicative.
 Require Import Classes.Monad.
 Require Import Types.Result.
 Require Import Types.Stores.
 Require Import Types.Maps.
 Require Import Instances.Monad.
+Require Import FunctionalExtensionality.
 
-Definition State (A : Type)         := Maybe (state (total_map cvalue) A).
-Definition AbstractState (A : Type) := AbstractMaybe (state (total_map avalue) A).
-
-(*
-Definition return_state {A : Type} (x : A) : State A :=
-  fun st => returnR x st.
-Arguments return_state [_] _.
-
-Definition bind_state {A B : Type} (m : State A) (f : A -> State B) 
-    : State B :=
-  fun st => match m st with
-            | returnR x st' => f x st'
-            | crashed => crashed 
-            | exception st' => exception st'
-            end.
-Arguments bind_state [_ _] _ _.
-
-Definition get : State store := fun st => returnR st st.
-
-Definition put (st' : store) : State unit := 
-  fun st => returnR tt st'.
-  
-
-Definition AbstractState (A : Type) :=
-  abstract_store -> abstract_result A abstract_store.
-
-Definition return_state_abstract {A : Type} (x : A) : AbstractState A :=
-  fun st => returnRA x st.
-Arguments return_state_abstract [_] _.
-
-Definition bind_state_abstract {A B : Type}
-  (m : AbstractState A) (f : A -> AbstractState B) : AbstractState B :=
-  fun st => match m st with
-            | returnRA x st' => f x st'
-            | crashedA => crashedA 
-            | exceptionA st' => exceptionA st' 
-            | exceptionOrReturn x st' => match (f x st') with 
-                                         | returnRA x' st'' => 
-                                             exceptionOrReturn x' 
-                                                              (join_op st' st'')
-                                         | crashedA => crashedA 
-                                         | exceptionA st'' => 
-                                             exceptionA (join_op st' st'')
-                                         | exceptionOrReturn x' st'' => 
-                                             exceptionOrReturn x' 
-                                                (join_op st' st'')
-                                         end
-            end.
-Arguments bind_state_abstract [_ _] _ _.
-*)
-
-Section abstract_state_joinable.
-Context {A : Type} `{Joinable A}.
+Definition ConcreteState := MaybeT (StateT store Maybe ).
 
 
-Definition join_state_abstract
-  (st1 st2 : AbstractState A) : AbstractState A :=
-  match st1 with
-  | NoneA _ => NoneA _
-  | JustA _ x => match st2 with
-                 | NoneA _ => NoneA _
-                 | JustA _ y => JustA _ (join_op x y)
-                 | JustOrNoneA _ y => JustOrNoneA _ (join_op x y)
-                 end
-  | JustOrNoneA _ x => match st2 with
-                       | NoneA _ => NoneA _
-                       | JustA _ y | JustOrNoneA _ y => 
-                           JustOrNoneA _ (join_op x y)
-                       end
-  end.
+Definition AbstractState := 
+  MaybeAT (StateT abstract_store Maybe).
 
-Lemma join_state_abstract_upperbound_left : forall st st',
-  preorder st (join_state_abstract st st').
-Proof.
-  intros. destruct st, st'; constructor; apply join_upper_bound_left.
-Qed.
+Section preorder.
+  Context {A} `{PreorderedSet A}.
 
-Lemma join_state_abstract_upperbound_right : forall st st',
-  preorder st' (join_state_abstract st st').
-Proof.
-  intros. destruct st, st'; constructor; apply join_upper_bound_right.
-Qed.
-
-Global Instance abstract_state_joinable : Joinable (AbstractState A) := 
-{
-  join_op := join_state_abstract;
-  join_upper_bound_left := join_state_abstract_upperbound_left;
-  join_upper_bound_right := join_state_abstract_upperbound_right;
-}.
-
-End abstract_state_joinable.
+  Global Instance preorder_abstract_state : PreorderedSet (AbstractState A).
+  Proof.
+    apply statet_preorder.
+  Defined.
+End preorder.
 
 
