Base.v
@@ -1,5 +1,6 @@
 Require Export Utf8.
 Require Import Program.Basics.
+Require Import FunctionalExtensionality.
 
 Create HintDb soundness.
 
@@ -9,4 +10,34 @@ Notation "f '$' x" := (f x)
   (at level 20, right associativity, only parsing).
 
 Definition id := fun {A : Type} (a : A) => a.
+
+Lemma id_refl : forall {A : Type} (x : A), id x = x.
+Proof. reflexivity. Qed.
+
+Hint Rewrite @id_refl : soundness.
+
 Notation "f ∘ g" := (compose g f).
+
+Ltac ext := let x := fresh "x" in extensionality x.
+
+Ltac unmatch x :=
+  match x with
+  | context [match ?y with _ => _ end] => unmatch y
+  | _ => destruct x eqn:?
+  end.
+
+Ltac destr :=
+  match goal with
+  | [ |- context [match ?x with _ => _ end]] => unmatch x
+  | [ |- context [let (_, _) := ?x in _]] => destruct x eqn:?
+  | H : (_ , _) = (_, _) |- _ => inv H; subst
+  end.
+
+Ltac simplify := simpl; intros; repeat ext; try destr.
+
+Ltac simple_solve := 
+  repeat (simplify; autorewrite with soundness + autounfold with soundness);
+  unfold compose;
+  try (congruence + reflexivity).
+
+Global Set Typeclasses Depth 5.
