Instances/Except/AbstractException.v
@@ -5,16 +5,19 @@ Require Import Types.Stores.
 Require Import Types.Result.
 Require Import Types.State.
 Require Import Instances.Monad.
+Require Import Classes.Monad.
+Require Import Classes.Applicative.
 
 Definition eval_catch_abstract 
   (st1 st2 : AbstractState unit) : AbstractState unit :=
-  match st1 with
-  | NoneA _ => st2
-  | JustA _ st => JustA _ st
-  | JustOrNoneA _ st => join_op st1 st2
-  end.
+  bindM (M:=State abstract_store) st1 (fun x => match x with
+                                       | JustA _ => st1
+                                       | JustOrNoneA _ => st2
+                                       | NoneA => st2
+                                       end).
 
-Definition fail_abstract : AbstractState unit := NoneA _.
+Definition fail_abstract : AbstractState unit := 
+  pure (F:=State abstract_store) NoneA.
 
 Instance except_abstract : Except AbstractState := 
 {
