Instances/Except/ConcreteException.v
@@ -3,16 +3,19 @@ Require Import Types.Result.
 Require Import Classes.Except.
 Require Import Types.Stores.
 Require Import Instances.Monad.
+Require Import Classes.Monad.
+Require Import Classes.Applicative.
 
-Definition eval_catch (st1 st2 : State unit) : State unit :=
-  match st1 with
-  | None _ => st2
-  | Just _ x => st1
-  end.
 
-Definition fail : State unit := None _.
+Definition eval_catch (st1 st2 : ConcreteState unit) : ConcreteState unit :=
+  bindM (M:=State store) st1 (fun m => match m with
+                            | Just _ => st1
+                            | None => st2
+                            end).
+                  
+Definition fail : ConcreteState unit := pure None.
 
-Instance except_concrete : Except State := {
+Instance except_concrete : Except ConcreteState := {
   throw := fail;
   trycatch := eval_catch;
 }.
