Instances/IsBool/Boolean.v
@@ -5,30 +5,30 @@ Require Import Types.State.
 Require Import Types.Stores.
 Require Import Types.Result.
 Require Import Instances.Monad.
+Require Import Classes.Applicative.
 
-Definition ensure_bool (v : cvalue) : State bool :=
+Definition ensure_bool (v : cvalue) : ConcreteState bool :=
   match v with
-  | VBool b => Just _ (returnM b)
-  | _ => None _
+  | VBool b => pure_maybeT _ (pure b)
+  | _ => pure None
   end.
 
-Definition build_boolean (b : bool) : State cvalue :=
-  Just _ (returnM (VBool b)).
+Definition build_boolean (b : bool) : ConcreteState cvalue :=
+  pure_maybeT _ (pure (VBool b)).
 
-Definition extract_boolean (b : bool) : State bool :=
-  Just _ (returnM b).
+Definition extract_boolean (b : bool) : ConcreteState bool :=
+  pure_maybeT _ (pure b).
 
-Definition andbM (b c : bool) : State bool := 
-  Just _ (returnM (andb b c)).
+Definition andbM (b c : bool) : ConcreteState bool := 
+  pure_maybeT _ (pure (andb b c)).
 
-Definition negbM (b : bool) : State bool := 
-  Just _ (returnM (negb b)).
+Definition negbM (b : bool) : ConcreteState bool := 
+  pure_maybeT _ (pure (negb b)).
 
-Definition eval_if {A} (b : bool) (st1 st2 : State A) : State A :=
+Definition eval_if {A} (b : bool) (st1 st2 : ConcreteState A) : ConcreteState A :=
   if b then st1 else st2.
 
-
-Instance boolean_type : IsBool State cvalue bool :=
+Instance boolean_type : IsBool ConcreteState cvalue bool :=
 {
   ensure_bool := ensure_bool;
   build_bool := build_boolean;
