Instances/IsNat/Interval.v
@@ -6,27 +6,28 @@ Require Import Types.Interval.
 Require Import Types.Result.
 Require Import Types.State.
 Require Import Instances.Monad.
+Require Import Classes.Applicative.
 
 Definition extract_interval (n : nat) : AbstractState interval := 
-    JustA _ (returnM (n, n)).
+    pure_maybeAT _ (pure (n, n)).
 
 Definition ensure_interval (v : avalue) : AbstractState interval :=
   match v with
-  | VInterval i => JustA _ (returnM i)
-  | _ => NoneA _
+  | VInterval i => pure_maybeAT _ (pure i)
+  | _ => pure NoneA 
   end.
 
 Definition iplusM (i j : interval) : AbstractState interval := 
-  JustA _ (returnM (iplus i j)).
+  pure_maybeAT _ (pure (iplus i j)).
 Definition imultM (i j : interval) : AbstractState interval :=
-  JustA _ (returnM (imult i j)).
+  pure_maybeAT _ (pure (imult i j)).
 Definition ieqM (i j : interval) : AbstractState abstr_bool :=
-  JustA _ (returnM (ieqb i j)).
+  pure_maybeAT _ (pure (ieqb i j)).
 Definition ileM (i j : interval) : AbstractState abstr_bool := 
-  JustA _ (returnM (ileqb i j)).
+  pure_maybeAT _ (pure (ileqb i j)).
 
 Definition build_interval (i : interval) : AbstractState avalue :=
-  JustA _ (returnM (VInterval i)).  
+  pure_maybeAT _ (pure (VInterval i)).  
 
 Global Instance isnat_interval : 
   IsNat AbstractState avalue abstr_bool interval := 
