Instances/Store/AbstractStore.v
@@ -7,25 +7,3 @@ Require Import Types.State.
 Require Import Types.Stores.
 Require Import Instances.Monad.
 
-Definition abstract_store_top : abstract_store :=
-  fun _ => VTop.
-Definition abstract_store_bottom : abstract_store :=
-  fun _ => VBottom.
-Definition abstract_store_join
-    (ast1 ast2 : abstract_store) : abstract_store :=
-  fun x => VTop.
-
-Compute (AbstractState avalue).
-
-Definition abstract_store_get (x : string) : AbstractState avalue := 
-  JustA _ (fun st : (total_map avalue) => (st x, st)).
-
-Definition abstract_store_put 
-  (x : string) (v : avalue) : 
-  AbstractState unit :=
-  JustA _ (fun st => (tt, (t_update st x v))).
-
-Instance store_abstract : Store AbstractState avalue := {
-  get := abstract_store_get;
-  put := abstract_store_put;
-}.
